update link layer for sload. simulate proof is admitted

RocqOfRust/revm/revm_interpreter/instructions/simulate/host/sload.v
@@ -1,17 +1,23 @@
 Require Import simulate.RocqOfRust.
 Require Import alloy_primitives.links.aliases.
 Require Import core.links.array.
+Require Import core.links.result.
 Require Import revm.revm_context_interface.links.host.
 Require Import revm.revm_context_interface.links.journaled_state.
 Require Import revm.revm_context_interface.simulate.host.
-Require Import revm.revm_interpreter.gas.simulate.calc.
+Require Import revm.revm_interpreter.gas.simulate.constants.
 Require Import revm.revm_interpreter.instructions.links.host.sload.
 Require Import revm.revm_interpreter.instructions.simulate.macros.
+Require Import revm.revm_interpreter.links.instruction_context.
+Require Import revm.revm_interpreter.links.gas.
 Require Import revm.revm_interpreter.links.interpreter.
 Require Import revm.revm_interpreter.links.instruction_result.
 Require Import revm.revm_interpreter.links.interpreter_types.
 Require Import revm.revm_interpreter.simulate.gas.
+Require Import revm.revm_interpreter.simulate.interpreter.
 Require Import revm.revm_interpreter.simulate.interpreter_types.
+Require Import revm.revm_primitives.links.hardfork.
+Require Import revm.revm_primitives.simulate.hardfork.
 
 Definition sload
     {WIRE H : Set} `{Link WIRE} `{Link H}
@@ -25,30 +31,63 @@ Definition sload
   popn_top_macro interpreter 0
     (fun interpreter => (interpreter, host)) (fun _ index_stub interpreter =>
   let index := index_stub.(RefStub.projection) interpreter.(Interpreter.stack) in
-  let target_address :=
-    IInterpreterTypes.(InterpreterTypes.InputsTrait_for_Input).(InputTraits.target_address)
-      interpreter.(Interpreter.input) in
-  let '(value_opt, host) := IHost.(Host.sload) host target_address index in
-  match value_opt with
-  | None =>
-    let control :=
-      IInterpreterTypes.(InterpreterTypes.LoopControl_for_Control).(LoopControl.set_instruction_result)
-        interpreter.(Interpreter.control)
-        instruction_result.InstructionResult.FatalExternalError in
-    (interpreter <| Interpreter.control := control |>, host)
-  | Some value =>
   let spec_id :=
     IInterpreterTypes.(InterpreterTypes.RuntimeFlag_for_RuntimeFlag).(RuntimeFlag.spec_id)
       interpreter.(Interpreter.runtime_flag) in
+  let target_address :=
+    IInterpreterTypes.(InterpreterTypes.InputsTrait_for_Input).(InputTraits.target_address)
+      interpreter.(Interpreter.input) in
+  let gas :=
+    if Impl_SpecId.is_enabled_in spec_id SpecId.BERLIN then
+      WARM_STORAGE_READ_COST
+    else if Impl_SpecId.is_enabled_in spec_id SpecId.ISTANBUL then
+      ISTANBUL_SLOAD_GAS
+    else if Impl_SpecId.is_enabled_in spec_id SpecId.TANGERINE then
+      200
+    else
+      50 in
   gas_macro interpreter
-    (calc.sload_cost spec_id value.(StateLoad.is_cold))
+    gas
     (fun interpreter => (interpreter, host)) (fun interpreter =>
+  if Impl_SpecId.is_enabled_in spec_id SpecId.BERLIN then
+    let skip_cold :=
+      interpreter.(Interpreter.gas).(Gas.remaining).(Integer.value) <?
+      COLD_SLOAD_COST_ADDITIONAL.(Integer.value) in
+    let '(value_result, host) :=
+      IHost.(Host.sload_skip_cold_load) host target_address index skip_cold in
+    match value_result with
+    | Result.Ok value =>
+        if value.(StateLoad.is_cold) then
+          gas_macro interpreter COLD_SLOAD_COST_ADDITIONAL
+            (fun interpreter => (interpreter, host)) (fun interpreter =>
+          let stack :=
+            index_stub.(RefStub.injection)
+              interpreter.(Interpreter.stack)
+              value.(StateLoad.data) in
+          (interpreter <| Interpreter.stack := stack |>, host))
+        else
+          let stack :=
+            index_stub.(RefStub.injection)
+              interpreter.(Interpreter.stack)
+              value.(StateLoad.data) in
+          (interpreter <| Interpreter.stack := stack |>, host)
+    | Result.Err LoadError.ColdLoadSkipped =>
+        (halt_oog interpreter, host)
+    | Result.Err LoadError.DBError =>
+        (halt_fatal interpreter, host)
+    end
+  else
+  let '(value_opt, host) := IHost.(Host.sload) host target_address index in
+  match value_opt with
+  | None =>
+      (halt_fatal interpreter, host)
+  | Some value =>
   let stack :=
     index_stub.(RefStub.injection)
       interpreter.(Interpreter.stack)
       value.(StateLoad.data) in
-  (interpreter <| Interpreter.stack := stack |>, host))
-  end).
+  (interpreter <| Interpreter.stack := stack |>, host)
+  end)).
 
 Lemma sload_eq
     {WIRE H : Set} `{Link WIRE} `{Link H}
@@ -65,10 +104,14 @@ Lemma sload_eq
     (host : H) :
   let ref_interpreter := make_ref 0 in
   let ref_host := make_ref (A := H) 1 in
+  let context := {|
+    instruction_context.InstructionContext.interpreter := ref_interpreter;
+    instruction_context.InstructionContext.host := ref_host;
+  |} in
   let result := sload interpreter host in
   {{
     SimulateM.eval_f
-      (run_sload run_InterpreterTypes_for_WIRE run_Host_for_H ref_interpreter ref_host)
+      (run_sload run_InterpreterTypes_for_WIRE run_Host_for_H context)
       [interpreter; host]%stack 🌲
     (
       Output.Success tt,
@@ -76,47 +119,4 @@ Lemma sload_eq
     )
   }}.
 Proof.
-  with_strategy transparent [run_sload] unfold sload, run_sload; cbn.
-  unfold popn_top_macro.
-  s. {
-    apply InterpreterTypesEq.
-  }
-  s; destruct _.(StackTrait.popn_top) as [[[]|] ?stack']; cbn. 2: {
-    s. {
-      apply InterpreterTypesEq.
-    }
-    s.
-  }
-  s. {
-    apply InterpreterTypesEq.
-  }
-  s. {
-    apply HostEq.
-  }
-  destruct _.(Host.sload) as [[value|] ?host]; cbn. 2: {
-    s. {
-      apply InterpreterTypesEq.
-    }
-    s.
-  }
-  s. {
-    apply InterpreterTypesEq.
-  }
-  unfold gas_macro.
-  s. {
-    apply InterpreterTypesEq.
-  }
-  s. {
-    apply calc.sload_cost_eq.
-  }
-  s. {
-    apply Impl_Gas.record_cost_eq.
-  }
-  destruct Impl_Gas.record_cost; cbn.
-  { s. }
-  { s. {
-      apply InterpreterTypesEq.
-    }
-    s.
-  }
-Qed.
+Admitted.
